proof of the wf of mpo which is compatible with nested permutations

mpo.v
@@ -10,7 +10,7 @@
 Require Import List Wellfounded Relations Permutation Utf8.
 Import ListNotations.
 
-Require Import mso.
+Require Import utils acc perm_eq mso.
 
 Set Implicit Arguments.
 
@@ -19,80 +19,9 @@ Set Implicit Arguments.
 
    http://www.lsv.ens-cachan.fr/Publis/PAPERS/PDF/JGL-mfcs13.pdf *)
 
-#[local] Notation "x ∈ l" := (In x l) (at level 70, no associativity, format "x  ∈  l").
-#[local] Notation "l ~ₚ m" := (@Permutation _ l m) (at level 70, no associativity, format "l  ~ₚ  m").
 #[local] Reserved Notation "l ~ₜ m" (at level 70, no associativity, format "l  ~ₜ  m").
-#[local] Notation "R ⁻¹" := (λ x y, R y x) (at level 1, left associativity, format "R ⁻¹").
-
-Section lex2.
-
-  (* An accessibility principle for the lexicographic product 
-     This one is somewhat new compared to the above reference
-     and allows for a clearer (even straightforward) proof 
-     of Acc_mpo_node below *)
-
-  Variables (X Y : Type) (R : X → X → Prop) (T : Y → Y → Prop).
-
-  Unset Elimination Schemes.
-
-  Inductive lex2 : X*Y → X*Y → Prop :=
-    | lex2_left  x₁ x₂ y₁ y₂ : R x₁ x₂ → lex2 (x₁,y₁) (x₂,y₂)
-    | lex2_right x y₁ y₂ :     T y₁ y₂ → lex2 (x,y₁) (x,y₂).
-
-  Set Elimination Schemes.
-
-  Hint Constructors lex2 : core.
-
-  Fact lex2_inv p q :
-      lex2 p q 
-    ↔ match p, q with
-      | (x₁,y₁), (x₂,y₂) => R x₁ x₂ ∨ x₁ = x₂ ∧ T y₁ y₂
-      end.
-  Proof.
-    split.
-    + intros []; auto.
-    + revert p q; intros [] [] [ | (<- & ?) ]; auto.
-  Qed.
-
-  Section Acc_lex2.
-
-    (* When proving a property for pairs
-       (x,y) s.t. Acc R x and Acc T y, we can
-       assume that it already holds for (x',y')
-       which are lex2-less as well as Acc(essible) *)
-
-    Variables (P : X → Y → Prop)
-              (HP : ∀ x₂ y₂, Acc R x₂
-                           → Acc T y₂
-                           → (∀ x₁ y₁, Acc R x₁
-                                     → Acc T y₁
-                                     → lex2 (x₁,y₁) (x₂,y₂)
-                                     → P x₁ y₁) 
-                           → P x₂ y₂).
-
-    Hint Resolve Acc_inv : core.
-
-    Theorem Acc_lex2 x y : Acc R x → Acc T y → P x y.
-    Proof.
-      intros Hx Hy; revert Hx y Hy.
-      do 2 induction 1.
-      apply HP.
-      1,2: constructor; auto.
-      intros ? ? ? ? [ | (<- & ?) ]%lex2_inv; auto.
-    Qed.
-
-  End Acc_lex2.
-
-End lex2.
-
-Fact fold_right_conj X (P : X → Prop) l :
-  fold_right (λ x, and (P x)) True l ↔ ∀x, x ∈ l → P x.
-Proof.
-  rewrite <- Forall_forall.
-  induction l; simpl.
-  + split; constructor.
-  + now rewrite Forall_cons_iff, IHl.
-Qed.
+#[local] Reserved Notation "x ⊏ₜ y" (at level 70, no associativity, format "x  ⊏ₜ  y").
+#[local] Reserved Notation "'⟨' x '|' l '⟩ₜ'" (at level 0, l at level 200, format "⟨ x | l ⟩ₜ").
 
 Section multiset_path_ordering.
 
@@ -105,13 +34,15 @@ Section multiset_path_ordering.
   Inductive term := node : X → list term → term.
 
   Set Elimination Schemes.
+  
+  Notation "⟨ f | l ⟩ₜ" := (node f l).
 
   Section term_ind.
 
     (* Induction principle for rose trees *)
 
     Variables (P : term → Prop)
-              (HP : ∀ f l, (∀t, t ∈ l → P t) → P (node f l)).
+              (HP : ∀ f l, (∀t, t ∈ l → P t) → P ⟨f|l⟩ₜ).
     
     Fixpoint term_ind t : P t.
     Proof.
@@ -136,10 +67,10 @@ Section multiset_path_ordering.
 
     Fixpoint term_fall t :=
       match t with
-      | node f l => P f ∧ fold_right (λ p, and (term_fall p)) True l
+      | ⟨f|l⟩ₜ => P f ∧ fold_right (λ p, and (term_fall p)) True l
       end.
 
-    Fact term_fall_fix f l : term_fall (node f l) ↔ P f ∧ ∀t, t ∈ l → term_fall t.
+    Fact term_fall_fix f l : term_fall ⟨f|l⟩ₜ ↔ P f ∧ ∀t, t ∈ l → term_fall t.
     Proof. rewrite <- fold_right_conj; easy. Qed.
 
     (* And its associated induction principle *)
@@ -150,7 +81,7 @@ Section multiset_path_ordering.
                 (HQ : ∀ f l, P f
                            → (∀t, t ∈ l → term_fall t)
                            → (∀t, t ∈ l → Q t)
-                           → Q (node f l)).
+                           → Q ⟨f|l⟩ₜ).
 
       Fact term_fall_ind t : term_fall t → Q t.
       Proof. induction t; intros []%term_fall_fix; apply HQ; eauto. Qed.
@@ -161,147 +92,187 @@ Section multiset_path_ordering.
 
   (* t(erm)perm are nested permutations on terms, ie one can permute
      sons, but sons themselves can be internaly permuted etc ... 
-     so f[x[a,b],y] ~ₜ f[y,x[b,a]] for instance  *)
+     so f[g[a,b],h] ~ₜ f[h,g[b,a]] for instance  *)
   Inductive tperm : term → term → Prop :=
     | tperm_intro f l m : perm_eq tperm l m
-                        → tperm (node f l) (node f m).
+                        → ⟨f|l⟩ₜ ~ₜ ⟨f|m⟩ₜ
+  where "s ~ₜ t" := (tperm s t).
 
   Hint Constructors tperm : core.
-
-  Infix "~ₜ" := tperm.
 
   Fact tperm_inv s t :
        s ~ₜ t
      → match s, t with
-       | node f l, node g m =>
-          f = g ∧ perm_eq tperm l m
+       | ⟨f|l⟩ₜ, ⟨g|m⟩ₜ => f = g ∧ perm_eq tperm l m
       end.
   Proof. destruct 1; eauto. Qed.
 
-  Hint Resolve perm_eq_refl perm_eq_sym perm_eq_trans : core.
+  Fact tperm_xchg {l k} : perm_eq tperm l k → ∃p, l ~ₚ p ∧ Forall2 tperm p k.
+  Proof. apply perm_eq_xchg. Qed.
 
-  Fact tperm_xchg {l m k} :
-      Forall2 tperm l m
-    → m ~ₚ k 
-    → ∃p, l ~ₚ p 
-        ∧ Forall2 tperm p k.
-  Proof. apply Forall2_perm_xchg. Qed.
+  (** tperm is an equivalence relation *)
 
-  (* tperm is an equivalence relation *)
+  (* because of the nesting, we need relativized versions *)
+  Hint Resolve perm_eq_refl_rel perm_eq_sym_rel perm_eq_trans_rel : core.
 
-  Fact tperm_refl t : t ~ₜ t.
-  Proof. induction t; eauto. Qed. 
+  Fact tperm_refl : reflexive tperm.
+  Proof. intro t; induction t; eauto. Qed. 
 
-  Fact tperm_sym s t : s ~ₜ t → t ~ₜ s.
-  Proof. revert t; induction s; intros [] []%tperm_inv; subst; eauto. Qed.
+  Fact tperm_sym : symmetric tperm.
+  Proof. intro s; induction s; intros [] []%tperm_inv; subst; eauto. Qed.
 
-  Fact tperm_trans r s t : r ~ₜ s → s ~ₜ t → r ~ₜ t.
-  Proof. revert r t; induction s; intros [] [] []%tperm_inv []%tperm_inv; subst; eauto. Qed.
+  Fact tperm_trans : transitive tperm.
+  Proof. intros r s; revert r; induction s; intros [] [] []%tperm_inv []%tperm_inv; subst; eauto. Qed.
 
   Hint Resolve tperm_refl tperm_sym tperm_trans : core.
+
+  Section example.
+  
+    Variables (f g c d e : X).
+    
+    Let a := ⟨c|[]⟩ₜ.
+    Let b := ⟨d|[]⟩ₜ.
+    Let h := ⟨e|[]⟩ₜ.
+    Let t1 := ⟨f|[⟨g|[a;b]⟩ₜ;h]⟩ₜ.
+    Let t2 := ⟨f|[h;⟨g|[b;a]⟩ₜ]⟩ₜ.
+    
+    Local Fact tperm_example : t1 ~ₜ t2.
+    Proof.
+      constructor.
+      constructor 1 with [⟨g|[b; a]⟩ₜ;h].
+      2: apply Permutation_app_comm with (l := [_]) (l' := [_]).
+      repeat constructor; auto.
+      constructor 1 with [a;b].
+      2: apply Permutation_app_comm with (l := [_]) (l' := [_]).
+      repeat constructor; auto.
+    Qed.
+
+  End example.
 
   (** The multiset path ordering *)
 
   Variables (R : X → X → Prop).
 
-  (* mpo is is a nested form of mso *)
+  (* mpo containing mso mpo tperm is a nested form of mso *)
   Inductive mpo : term → term → Prop :=
     | mpo_in_lt s t g m :   t ∈ m
-                          → mpo s t
-                          → mpo s (node g m)
+                          → s ⊏ₜ t
+                          → s ⊏ₜ ⟨g|m⟩ₜ
     | mpo_in_eq s t g m :   t ∈ m
                           → s ~ₜ t
-                          → mpo s (node g m)
-    | mpo_lt f l g m :      (∀r, r ∈ l → mpo r (node g m))
+                          → s ⊏ₜ ⟨g|m⟩ₜ
+    | mpo_lt f l g m :      (∀t, t ∈ l → t ⊏ₜ ⟨g|m⟩ₜ)
                           → R f g
-                          → mpo (node f l) (node g m)
-    | mpo_eq l g m :        (∀r, r ∈ l → mpo r (node g m))
+                          → ⟨f|l⟩ₜ ⊏ₜ ⟨g|m⟩ₜ
+    | mpo_eq l g m :        (∀t, t ∈ l → t ⊏ₜ ⟨g|m⟩ₜ)
                           → mso mpo tperm l m
-                          → mpo (node g l) (node g m).
+                          → ⟨g|l⟩ₜ ⊏ₜ ⟨g|m⟩ₜ
+  where "s ⊏ₜ t" := (mpo s t). 
+
+  Hint Constructors mpo : core.
 
   Fact mpo_inv s t :
       mpo s t 
     → match s, t with
-      | node f l, node g m =>
-          (∃r, r ∈ m ∧ mpo s r)
+      | ⟨f|l⟩ₜ, ⟨g|m⟩ₜ =>
+          (∃r, r ∈ m ∧ s ⊏ₜ r)
         ∨ (∃r, r ∈ m ∧ s ~ₜ r)
-        ∨ (R f g ∧ ∀r, r ∈ l → mpo r (node g m))
-        ∨ (f = g ∧ mso mpo tperm l m ∧ ∀r, r ∈ l → mpo r (node g m))
+        ∨ (R f g ∧ ∀r, r ∈ l → r ⊏ₜ t)
+        ∨ (f = g ∧ mso mpo tperm l m ∧ ∀r, r ∈ l → r ⊏ₜ t)
       end.
   Proof.
     destruct 1; eauto.
-    + destruct s; eauto.
-    + destruct s; eauto.
-    + do 3 right; auto.
+    1,2: destruct s; eauto.
+    do 3 right; auto.
   Qed.
 
-  Hint Constructors tperm : core.
+  Hint Resolve Permutation_in Permutation_sym : core.
 
-  Fact tperm_mpo_right r s t : s ~ₜ t → mpo r s → mpo r t.
+  (** We first show that ~ₜ is a congruence for mpo.
+      This involves nested inductions, hence the 
+      relativized form of mso_perm_r *)
+
+  (* This one was the hardest lemma to get right !!
+      We need the relativized form of mso_perm_r *)
+  Lemma mpo_tperm_right s t : s ~ₜ t → ∀r, r ⊏ₜ s → r ⊏ₜ t.
   Proof.
-    revert r t.
-    induction s as [ g l IHs ];
-    induction r as [ f p IHr ].
-    intros [ h m ].
-    intros (<- & Hlm)%tperm_inv.
+    (* By induction on s then r *)
+    intros H r; revert s r t H.
+    intro s; induction s as [ g l IHl ].
+    intro r; induction r as [ f p IHp ].
+    intros [ ? m ] (<- & Hlm)%tperm_inv.
     intros [ (r & H3 & H4) 
          | [ (r & H3 & H4)
          | [ (H3 & H4)
            | (<- & H3 & H4) ]
             ] ]%mpo_inv.
-    + destruct (tperm_xchg H1 H2) as (u & H5 & H6).
-      destruct Forall2_In_inv
-        with (1 := H6) (x := r)
-        as (v & H7 & H8); eauto.
-      constructor 1 with v; eauto.
-    + destruct (tperm_xchg H1 H2) as (u & H5 & H6).
-      destruct Forall2_In_inv
-        with (1 := H6) (x := r)
-        as (v & H7 & H8); eauto.
-      constructor 2 with v; eauto.
+    + apply tperm_xchg in Hlm as (u & H5 & H6).
+      destruct Forall2_In_inv with (1 := H6) (x := r) as (? & []); eauto.
+    + apply tperm_xchg in Hlm as (u & H5 & H6).
+      destruct Forall2_In_inv with (1 := H6) (x := r) as (? & []); eauto.
     + constructor 3; eauto.
     + constructor 4; eauto.
-      apply mso_perm_r with (1 := H2).
-      revert H3.
-      assert (forall x y z, x ∈ p → y ∈ l → z ∈ k → y ~ₜ z → mpo x y → mpo x z).
-      1: eauto. intros ? ? ? ? ? ?; apply IHs.
-  Admitted.
-
-  Fact tperm_Acc_mpo s t : s ~ₜ t → Acc mpo s → Acc mpo t.
-  Proof.
-    intros H1 H2; revert H2 t H1.
-    induction 1 as [ s _ IHs ]; intros t Hst.
-    constructor.
-    intros r Hr.
-    generalize (tperm_mpo_right (tperm_sym Hst) Hr); eauto.
+      (* We need a relativized form mso_perm_r_rel 
+         than can be applied recursively *)
+      revert H3; apply mso_perm_r_rel; eauto.
   Qed.
 
+  (* This one follows as a consequence *)
+  Lemma mpo_tperm_left r s t : r ~ₜ s → r ⊏ₜ t → s ⊏ₜ t.
+  Proof.
+    revert t r s.
+    intro t; induction t as [ g m IHm ].
+    intro r; induction r as [ f l IHl ].
+    intros [ ? p ] (<- & Hlm)%tperm_inv.
+    intros [ (r & H3 & H4) 
+         | [ (r & H3 & H4)
+         | [ (H3 & H4)
+           | (<- & H3 & H4) ]
+            ] ]%mpo_inv; eauto.
+    + constructor 3; auto.
+      apply perm_eq_sym in Hlm; auto.
+      intros r Hr.
+      destruct perm_eq_in_inv with (1 := Hlm) (2 := Hr) as (? & []); eauto.
+    + constructor 4; eauto.
+      * apply perm_eq_sym in Hlm; auto. 
+        intros r Hr.
+        destruct perm_eq_in_inv with (1 := Hlm) (2 := Hr) as (? & []); eauto.
+      * revert H3; apply mso_perm_l; auto.
+        apply mpo_tperm_right.
+  Qed.
+
+  (** Now we establish Accessibility by structural induction *)
+
+  Local Corollary tperm_Acc_mpo s t : s ~ₜ t → Acc mpo t → Acc mpo s.
+  Proof. intro; now apply Acc_lower_bounds, mpo_tperm_right. Qed.
+
   Hint Constructors lex2 : core.
-  Hint Resolve Acc_inv forall_Acc_mso : core.
+  Hint Resolve Acc_inv tperm_Acc_mpo forall_Acc_mso mpo_tperm_right : core.
 
   (* node f l inherits Acc(essibility) from that of f and of l *)
-  Local Lemma Acc_mpo_node : ∀ f l, Acc R f → Acc (mso mpo) l → Acc mpo (node f l).
+  Local Lemma Acc_mpo_node : ∀ f l, Acc R f → Acc (mso mpo tperm) l → Acc mpo ⟨f|l⟩ₜ.
   Proof.
-    (* We use Acc_lex2 induction for a straightforward proof 
-       The other essential property of of course 
+    (* We use Acc_lex2 induction for a straightforward proof
+       The other essential property is of course 
           Acc (mso T) l ↔ ∀x, x ∈ l → Acc T x applied to T := mpo *)
     apply Acc_lex2; intros g m Hg Hm IH.
-    rewrite Acc_mso_iff in Hm.
-    constructor; intros s.
-    induction s as [ f l IHl ].
+    rewrite Acc_mso_iff in Hm; eauto.
+    constructor.
+    intro s; induction s as [ f l IHl ].
     intros [ (? & [])
          | [ (? & [])
          | [ []
            | (<- & []) ] ] ]%mpo_inv; eauto.
-    + admit.
-    + apply IH; eauto.
+    all: apply IH; eauto.
   Qed.
 
   Hint Resolve Acc_mpo_node : core.
 
   (* Hence if all nodes are Acc(essible) then so is the tree *)
-  Lemma Acc_mpo_term_fall : ∀t, term_fall (Acc R) t → Acc mpo t.
-  Proof. apply term_fall_ind; auto. Qed.
+  Lemma Acc_mpo_term_fall t : term_fall (Acc R) t → Acc mpo t.
+  Proof. induction 1 using term_fall_ind; eauto. Qed.
+
+  (** We conclude with the well-foundedness result *)
 
   Hypothesis R_wf : well_founded R.
 
@@ -316,4 +287,6 @@ Section multiset_path_ordering.
   Proof. red; auto. Qed.
 
 End multiset_path_ordering.
+
+Check mpo_wf.
 
