acc.v
@@ -1,0 +1,73 @@
+(**************************************************************)
+(*   Copyright Dominique Larchey-Wendling [*]                 *)
+(*                                                            *)
+(*                             [*] Affiliation LORIA -- CNRS  *)
+(**************************************************************)
+(*      This file is distributed under the terms of the       *)
+(*        Mozilla Public License Version 2.0, MPL-2.0         *)
+(**************************************************************)
+
+Require Import Wellfounded Utf8.
+
+Fact Acc_lower_bounds X (R : X → X → Prop) x y : (∀u, R u x → R u y) → Acc R y → Acc R x.
+Proof. intros ? []; constructor; eauto. Qed. 
+
+Section lex2.
+
+  (* A double Acc induction principle for the lexicographic product 
+     This one is somewhat new compared to the above reference
+     and allows for a clearer (even straightforward) proof 
+     of Acc_mpo_node below *)
+
+  Variables (X Y : Type) (R : X → X → Prop) (T : Y → Y → Prop).
+
+  Unset Elimination Schemes.
+
+  Inductive lex2 : X*Y → X*Y → Prop :=
+    | lex2_left  x₁ x₂ y₁ y₂ : R x₁ x₂ → lex2 (x₁,y₁) (x₂,y₂)
+    | lex2_right x y₁ y₂ :     T y₁ y₂ → lex2 (x,y₁) (x,y₂).
+
+  Set Elimination Schemes.
+
+  Hint Constructors lex2 : core.
+
+  Fact lex2_inv p q :
+      lex2 p q 
+    ↔ match p, q with
+      | (x₁,y₁), (x₂,y₂) => R x₁ x₂ ∨ x₁ = x₂ ∧ T y₁ y₂
+      end.
+  Proof.
+    split.
+    + intros []; auto.
+    + revert p q; intros [] [] [ | (<- & ?) ]; auto.
+  Qed.
+
+  Section Acc_lex2.
+
+    (* When proving a property for pairs
+       (x,y) s.t. Acc R x and Acc T y, we can
+       assume that it already holds for (x',y')
+       which are lex2-less as well as Acc(essible) *)
+
+    Variables (P : X → Y → Prop)
+              (HP : ∀ x₂ y₂, Acc R x₂
+                           → Acc T y₂
+                           → (∀ x₁ y₁, Acc R x₁
+                                     → Acc T y₁
+                                     → lex2 (x₁,y₁) (x₂,y₂)
+                                     → P x₁ y₁) 
+                           → P x₂ y₂).
+
+    Hint Resolve Acc_inv Acc_intro : core.
+
+    Theorem Acc_lex2 x y : Acc R x → Acc T y → P x y.
+    Proof.
+      intros Hx Hy; revert Hx y Hy.
+      do 2 induction 1.
+      apply HP; auto.
+      intros ? ? ? ? [ | (<- & ?) ]%lex2_inv; auto.
+    Qed.
+
+  End Acc_lex2.
+
+End lex2.
