perm_eq.v
@@ -1,0 +1,126 @@
+(**************************************************************)
+(*   Copyright Dominique Larchey-Wendling [*]                 *)
+(*                                                            *)
+(*                             [*] Affiliation LORIA -- CNRS  *)
+(**************************************************************)
+(*      This file is distributed under the terms of the       *)
+(*        Mozilla Public License Version 2.0, MPL-2.0         *)
+(**************************************************************)
+
+Require Import List Permutation Relations Utf8.
+Import ListNotations.
+
+Require Import utils.
+
+Set Implicit Arguments.
+
+Section perm_eq.
+
+  Hint Resolve Permutation_app 
+               Permutation_sym
+               Permutation_trans
+               Permutation_in
+               Permutation_app_comm : core.
+
+  Hint Resolve Forall2_app Forall2_diag : core.
+
+  Variable (X : Type) (E : X → X → Prop).
+
+  Inductive perm_eq (l k : list X) : Prop :=
+    | perm_eq_intro m : Forall2 E l m → m ~ₚ k → perm_eq l k.
+
+  Hint Constructors perm_eq : core.
+  
+  Notation "l ~ₑ m" := (perm_eq l m) (at level 70, format "l  ~ₑ  m" ).
+
+  Fact perm_eq_in_inv l m x : l ~ₑ m → x ∈ l → ∃y, y ∈ m ∧ E x y.
+  Proof.
+    intros [ k H1 H2 ] Hx.
+    destruct (Forall2_In_inv _ H1 Hx) as (? & []); eauto.
+  Qed.
+
+  Fact perm_eq_xchg l m : l ~ₑ m → ∃p, l ~ₚ p ∧ Forall2 E p m.
+  Proof.
+    destruct 1 as [ k H1 H2 ].
+    apply (Forall2_perm_xchg H1 H2).
+  Qed.
+
+  (* We need relativized versions of refl-sym-trans to 
+     reason recursivively in the case of nesting of perm_eq *)
+
+  Fact perm_eq_refl_rel l : (∀x, x ∈ l → E x x) → l ~ₑ l.
+  Proof.
+    constructor 1 with l; auto.
+    rewrite <- Forall_forall in H.
+    induction H; eauto.
+  Qed.
+
+  Fact perm_eq_sym_rel l m :
+      (∀ x y, x ∈ l → y ∈ m → E x y → E y x)
+    → l ~ₑ m → m ~ₑ l.
+  Proof.
+    intros Hlm (p & H1 & H2%Forall2_xchg)%perm_eq_xchg.
+    constructor 1 with p; auto.
+    revert H2; apply Forall2_impl_dep; eauto.
+  Qed.
+
+  Fact perm_eq_trans_rel l m k : 
+      (∀ x y z, x ∈ l → y ∈ m → z ∈ k → E x y → E y z → E x z)
+    → l ~ₑ m → m ~ₑ k → l ~ₑ k.
+  Proof.
+    intros Hlmk.
+    intros (u & H1 & H2)%perm_eq_xchg.
+    destruct 1 as [ v H3 H4 ].
+    assert (Forall2 E u v) as Huv.
+    1: revert H2 H3; apply Forall2_trans_dep; eauto.
+    destruct (perm_Forall2_xchg H1 Huv) as (? & []); eauto.
+  Qed.
+
+  Fact perm_eq_app l m k p : l ~ₑ m → k ~ₑ p → l++k ~ₑ m++p.
+  Proof. do 2 destruct 1; eauto. Qed.
+
+  Fact perm_eq_app_comm_rel l m :
+      (∀x, x ∈ l → E x x)
+    → (∀x, x ∈ m → E x x)
+    → l++m ~ₑ m++l.
+  Proof. rewrite <- !Forall_forall; eauto. Qed.
+
+  Fact perm_eq_middle_inv l x r m : 
+      l++[x]++r ~ₑ m 
+    → ∃ l' y r', E x y 
+               ∧ m = l'++[y]++r' 
+               ∧ l++r ~ₑ l'++r'.
+  Proof.
+    destruct 1 as [ v (l1 & y & r1 & -> & H1 & H2 & H3)%Forall2_middle_inv_left 
+                    (l' & r' & -> & H)%Permutation_middle_inv ].
+    exists l', y, r'; eauto.
+  Qed.
+  
+  Hypothesis E_refl : reflexive E.
+  Hypothesis E_sym : symmetric E.
+  Hypothesis E_trans : transitive E.
+
+  Fact perm_eq_refl : reflexive perm_eq.
+  Proof. intro; apply perm_eq_refl_rel; auto. Qed.
+
+  Fact perm_eq_sym : symmetric perm_eq.
+  Proof. intros ? ?; apply perm_eq_sym_rel; auto. Qed.
+
+  Fact perm_eq_trans : transitive perm_eq.
+  Proof. intros ? ? ?; apply perm_eq_trans_rel; eauto. Qed.
+  
+  Fact perm_eq_app_comm l m : l++m ~ₑ m++l.
+  Proof. apply perm_eq_app_comm_rel; auto. Qed.
+
+  Fact perm_eq_middle l m r l' r' :
+      l++r ~ₑ l'++r'
+    → l++m++r ~ₑ l'++m++r'.
+  Proof.
+    intro.
+    do 2 apply (perm_eq_trans (perm_eq_app_comm _ _)), perm_eq_sym.
+    rewrite <- ! app_assoc.
+    apply perm_eq_app; auto using perm_eq_refl.
+    now do 2 apply (perm_eq_trans (perm_eq_app_comm _ _)), perm_eq_sym.
+  Qed.
+
+End perm_eq.
