utils.v
@@ -1,0 +1,154 @@
+(**************************************************************)
+(*   Copyright Dominique Larchey-Wendling [*]                 *)
+(*                                                            *)
+(*                             [*] Affiliation LORIA -- CNRS  *)
+(**************************************************************)
+(*      This file is distributed under the terms of the       *)
+(*        Mozilla Public License Version 2.0, MPL-2.0         *)
+(**************************************************************)
+
+Require Import List Permutation Relations Utf8.
+Import ListNotations.
+
+Set Implicit Arguments.
+
+#[global] Notation "x ∈ l" := (In x l) (at level 70, no associativity, format "x  ∈  l").
+#[global] Notation "l ~ₚ m" := (@Permutation _ l m) (at level 70, no associativity, format "l  ~ₚ  m").
+#[global] Notation "R ⁻¹" := (λ x y, R y x) (at level 1, left associativity, format "R ⁻¹").
+
+Arguments clos_trans {_}.
+Arguments clos_refl_trans {_}.
+Arguments reflexive {_}.
+Arguments symmetric {_}.
+Arguments transitive {_}.
+
+#[local] Hint Resolve in_cons in_eq in_elt in_or_app 
+                      Permutation_app_inv Permutation_app_middle Permutation_app
+                      Permutation_sym Permutation_trans : core.
+
+#[local] Hint Constructors clos_trans clos_refl_trans : core.
+
+Section utilities.
+
+  Variable (X : Type).
+
+  Implicit Types (x : X) (l : list X) (R : X → X → Prop) (P : X → Prop).
+
+  Fact cons_inj x y l m : x::l = y::m → x = y ∧ l = m.
+  Proof. now inversion 1. Qed.
+
+  (* _++[_]++_ is a better shape than _++_::_ for rewrites below *)
+  Fact in_split x m : x ∈ m → ∃ l r, m = l++[x]++r.
+  Proof. apply in_split. Qed.
+
+  Fact fold_right_conj P l : fold_right (λ x, and (P x)) True l ↔ ∀x, x ∈ l → P x.
+  Proof.
+    rewrite <- Forall_forall.
+    induction l; simpl.
+    + split; constructor.
+    + now rewrite Forall_cons_iff, IHl.
+  Qed.
+
+  Fact Permutation_middle_inv l x r m :
+    l++[x]++r ~ₚ m → ∃ l' r', m = l'++[x]++r' ∧ l++r ~ₚ l'++r'.
+  Proof.
+    intros H.
+    assert (x ∈ m) as (l' & r' & ->)%in_split; simpl; eauto.
+    apply Permutation_in with (1 := H); auto.
+  Qed.
+  
+  Fact clos_trans__clos_refl_trans R x y : clos_trans R x y → clos_refl_trans R x y.
+  Proof. induction 1; eauto. Qed. 
+  
+  Hint Resolve clos_trans__clos_refl_trans : core.
+
+  Fact clos_refl_trans__clos_trans R x y : clos_refl_trans R x y ↔ x = y ∨ clos_trans R x y.
+  Proof.
+    split.
+    + induction 1 as [ | | ? ? ? _ [] _ [] ]; subst; eauto.
+    + intros [ <- | ]; eauto.
+  Qed.
+
+  Fact clos_trans_inv_right R x z : clos_trans R x z ↔ ∃y, clos_refl_trans R x y ∧ R y z.
+  Proof. 
+    split.
+    + induction 1 as [ | ? ? ? ? _ _ (? & []) ]; eauto.
+    + intros (? & [ <- | ]%clos_refl_trans__clos_trans & H2); eauto.
+  Qed.
+
+End utilities.
+
+Fact Forall2_middle_inv_left X Y (R : X → Y → Prop) l x r m :
+  Forall2 R (l++[x]++r) m → ∃ l' y r', m = l'++[y]++r' ∧ R x y ∧ Forall2 R l l' ∧ Forall2 R r r'.
+Proof.
+  intros (l' & [ | y r' ] & H1 & H2 & ->)%Forall2_app_inv_l.
+  1: now inversion H2.
+  apply Forall2_cons_iff in H2 as (? & ?).
+  exists l', y, r'; auto.
+Qed.
+
+Fact Permutation_head_inv X (x : X) k m :
+    x::k ~ₚ m → ∃ l r, m = l++x::r ∧ k ~ₚ l++r.
+Proof.
+  intros H.
+  destruct (in_split x m) as (l & r & ->).
+  + apply Permutation_in with (1 := H); simpl; auto.
+  + exists l, r; split; auto.
+    now apply Permutation_cons_inv with x,
+          perm_trans with (1 := H), 
+          Permutation_sym,
+          Permutation_cons_app.
+Qed.
+
+Fact Forall2_xchg X Y (R : X → Y → Prop) l m : Forall2 R l m → Forall2 R⁻¹ m l.
+Proof. induction 1; eauto. Qed.
+
+Fact Forall2_impl_dep X Y (R T : X → Y → Prop) l m :
+  (∀ x y, x ∈ l → y ∈ m → R x y → T x y) → Forall2 R l m → Forall2 T l m.
+Proof.
+  intros H1 H2; revert H2 H1.
+  induction 1; simpl; intro; constructor; eauto.
+Qed.
+
+Fact Forall2_trans_dep X (R : X → X → Prop) l m k :
+    (∀ x y z, x ∈ l → y ∈ m → z ∈ k → R x y → R y z → R x z)
+  → Forall2 R l m
+  → Forall2 R m k
+  → Forall2 R l k.
+Proof.
+  intros H1 H2; revert H2 k H1.
+  induction 1 as [ | x y l m H1 H2 IH2 ]; intros k H3; auto.
+  + destruct k as [ | z k ]; [ now inversion 1 | ].
+    intros (H4 & H5)%Forall2_cons_iff.
+    constructor; eauto.
+    revert H5; apply IH2; eauto.
+Qed.
+
+Fact Forall2_In_inv X Y (R : X → Y → Prop) x l m :
+  Forall2 R l m → x ∈ l → ∃y, R x y ∧ y ∈ m.
+Proof.
+  induction 1 as [ | a b l m H1 H2 IH2 ].
+  + now inversion 1.
+  + intros [ <- | (? & [])%IH2 ]; eauto.
+Qed.
+
+Fact Forall2_perm_xchg [X Y] [E : X → Y → Prop] [l m k] :
+  Forall2 E l m → m ~ₚ k → ∃p, l ~ₚ p ∧ Forall2 E p k.
+Proof.
+  induction 1 as [ | s t l m H1 H2 IH2 ] in k |- *.
+  + intros ->%Permutation_nil; exists []; eauto.
+  + intros (k1 & k2 & -> & (p & ? & (l1 & l2 & ? & ? & ->)%Forall2_app_inv_r)%IH2)%Permutation_head_inv.
+    exists (l1++s::l2); split.
+    * now apply Permutation_cons_app.
+    * apply Forall2_app; auto.
+Qed.
+
+Fact Forall2_diag X (R : X → X → Prop) l : Forall (λ x, R x x) l → Forall2 R l l.
+Proof. induction 1; eauto. Qed.
+
+Fact perm_Forall2_xchg [X Y] [E : X → Y → Prop] [l m k] :
+  l ~ₚ m → Forall2 E m k → ∃p, Forall2 E l p ∧ p ~ₚ k.
+Proof.
+  intros H1%Permutation_sym H2%Forall2_xchg.
+  destruct (Forall2_perm_xchg H2 H1) as (? & ? & ?%Forall2_xchg); eauto.
+Qed.
